Completed up to anno term defs

src/Anno_Term_Defs.v
@@ -29,8 +29,11 @@ Inductive AnnoTerm :=
 | abseq: Range -> Split -> AnnoTerm -> AnnoTerm -> AnnoTerm
 | abpar: Range -> Split -> AnnoTerm -> AnnoTerm -> AnnoTerm.
 
+Inductive AnnoCopPhrase :=
+| anno_cop_phrase : Plc -> EvidenceT -> AnnoTerm -> AnnoCopPhrase.
+
 (* EvidenceT Type size *)
-Fixpoint esize (G : ASP_Type_Env) (t : AnnoTerm) (e : EvidenceT) 
+Fixpoint esize (G : GlobalContext) (e : EvidenceT) (t : AnnoTerm)
     : ResultT nat string :=
   match t with
   | aasp _ a => 
@@ -39,20 +42,20 @@ Fixpoint esize (G : ASP_Type_Env) (t : AnnoTerm) (e : EvidenceT)
     | _ => resultC 1
     end
   | aatt _ _ t1 => 
-    e' <- esize G t1 e ;;
+    e' <- esize G e t1 ;;
     resultC (2 + e')
   | alseq _ t1 t2 => 
-    e1 <- esize G t1 e ;;
-    e2 <- esize G t2 e ;;
+    e1 <- esize G e t1 ;;
+    e2 <- esize G e t2 ;;
     resultC (e1 + e2)
   
   | abseq _ _ t1 t2 => 
-    e1 <- esize G t1 e ;;
-    e2 <- esize G t2 e ;;
+    e1 <- esize G e t1 ;;
+    e2 <- esize G e t2 ;;
     resultC (2 + e1 + e2)
   | abpar _ _ t1 t2 => 
-    e1 <- esize G t1 e ;;
-    e2 <- esize G t2 e ;;
+    e1 <- esize G e t1 ;;
+    e2 <- esize G e t2 ;;
     resultC (2 + e1 + e2)
   end.
 
@@ -101,40 +104,76 @@ Proof.
   induction t''; intros; ff.
 Qed.
 
+(** eval (EvidenceT semantics) for annotated terms. *)
+
+Fixpoint aeval (G : GlobalContext) (p : Plc) (e : EvidenceT) (t : AnnoTerm) 
+    : ResultT EvidenceT string :=
+  match t with
+  | aasp _ x => eval G p e (asp x)
+  | aatt _ q x => aeval G q e x
+  | alseq _ t1 t2 => 
+      e1 <- aeval G p e t1 ;;
+      aeval G p e1 t2
+  | abseq _ s t1 t2 => 
+      e1 <- aeval G p (splitEv_T_l s e) t1 ;;
+      e2 <- aeval G p (splitEv_T_r s e) t2 ;;
+      resultC (split_evt e1 e2)
+  | abpar _ s t1 t2 => 
+      e1 <- aeval G p (splitEv_T_l s e) t1 ;;
+      e2 <- aeval G p (splitEv_T_r s e) t2 ;;
+      resultC (split_evt e1 e2)
+  end.
+
+
 (** This function annotates a term.  It feeds a natural number
     throughout the computation so as to ensure each event has a unique
     natural number. *)
-Fixpoint anno (G : ASP_Type_Env) (e : EvidenceT) (t: Term) (i:nat) 
-    : ResultT (nat * AnnoTerm) string :=
+Fixpoint anno (G : GlobalContext) (p : Plc) (e : EvidenceT) 
+    (t: Term) (i:nat) 
+    : ResultT (nat * AnnoTerm * EvidenceT) string :=
   match t with
   | asp x => 
     match x with
     | APPR => 
       match et_size G e with
       | errC s => errC s
-      | resultC n => resultC (S (i + n), aasp (i, S (i + n)) x)
+      | resultC n => 
+        let nterm := aasp (i, S i + n) x in
+        e' <- aeval G p e nterm ;;
+        resultC (S i + n, nterm, e')
       end
-    | _ => resultC (S i, aasp (i, S i) x)
+    | _ => 
+      let nterm := aasp (i, S i) x in
+      e' <- aeval G p e nterm ;;
+      resultC (S i, nterm, e')
     end
   
-  | att p x =>
-    '(j, a) <- anno G e x (S i) ;;
-    resultC (S j, aatt (i, S j) p a)
+  | att p' x =>
+    '(j, a, e') <- anno G p' e x (S i) ;;
+    let nterm := aatt (i, S j) p' a in
+    e' <- aeval G p e nterm ;;
+    resultC (S j, nterm, e')
 
   | lseq x y =>
-    '(j, a) <- anno G e x i ;;
-    '(k, b) <- anno G e y j ;;
-    resultC (k, alseq (i, k) a b)
+    '(j, a, e') <- anno G p e x i ;;
+    '(k, b, e'') <- anno G p e' y j ;;
+    let nterm := alseq (i, k) a b in
+    e' <- aeval G p e nterm ;;
+    resultC (k, nterm, e')
 
   | bseq s x y =>
-    '(j, a) <- anno G e x (S i) ;;
-    '(k, b) <- anno G e y j ;;
-    resultC (S k, abseq (i, S k) s a b)
+    '(j, a, e') <- anno G p (splitEv_T_l s e) x (S i) ;;
+    '(k, b, e'') <- anno G p (splitEv_T_r s e) y j ;;
+    let nterm := abseq (i, S k) s a b in
+    e' <- aeval G p e nterm ;;
+    resultC (S k, nterm, e')
 
   | bpar s x y =>
-    '(j, a) <- anno G e x (S i) ;;
-    '(k, b) <- anno G e y j ;;
-    resultC (S k, abpar (i, S k) s a b)
+    '(j, a, e') <- anno G p (splitEv_T_l s e) x (S i) ;;
+    '(k, b, e'') <- anno G p (splitEv_T_r s e) y j ;;
+    let nterm := abpar (i, S k) s a b in
+    e' <- aeval G p e nterm ;;
+    resultC (S k, nterm, e')
   end.
 
 Fixpoint unanno a :=
@@ -146,8 +185,8 @@ Fixpoint unanno a :=
   | abpar _ spl a1 a2 => bpar spl (unanno a1) (unanno a2)
   end.
 
-Lemma anno_unanno: forall e t t' i i' G,
-  anno G e t i = resultC (i', t') ->
+Lemma anno_unanno: forall e t t' i i' G p e',
+  anno G p e t i = resultC (i', t', e') ->
   unanno t' = t.
 Proof.
   intros.
@@ -155,188 +194,251 @@ Proof.
   induction t; intros; ffa using result_monad_unfold.
 Qed.
 
-(** eval (EvidenceT semantics) for annotated terms. *)
+Lemma anno_aeval : forall G t t' e e' p i i',
+  anno G p e t i = resultC (i', t', e') ->
+  aeval G p e t' = resultC e'.
+Proof.
+  induction t; simpl in *; intuition; ffa using result_monad_unfold.
+Qed.
 
-Fixpoint aeval (G : ASP_Type_Env) (cm : ASP_Compat_MapT) (t : AnnoTerm) 
-    (p : Plc) (e : EvidenceT) : ResultT EvidenceT string :=
-  match t with
-  | aasp _ x => eval G cm (asp x) p e
-  | aatt _ q x => aeval G cm x q e 
-  | alseq _ t1 t2 => 
-      e1 <- aeval G cm t1 p e ;;
-      aeval G cm t2 p e1 
-  | abseq _ s t1 t2 => 
-      e1 <- aeval G cm t1 p (splitEv_T_l s e) ;;
-      e2 <- aeval G cm t2 p (splitEv_T_r s e) ;;
-      resultC (split_evt e1 e2)
-  | abpar _ s t1 t2 => 
-      e1 <- aeval G cm t1 p (splitEv_T_l s e) ;;
-      e2 <- aeval G cm t2 p (splitEv_T_r s e) ;;
-      resultC (split_evt e1 e2)
+Lemma anno_eval : forall G t t' e e' p i i',
+  anno G p e t i = resultC (i', t', e') ->
+  eval G p e t = resultC e'.
+Proof.
+  induction t; simpl in *; intuition; ff;
+  result_monad_unfold; ff; 
+  try (ffa using result_monad_unfold; fail);
+  try (match goal with
+  | H: anno _ _ _ _ _ = _ |- _ => 
+    eapply anno_aeval in H as ?;
+    ffa
+  end; fail);
+  match goal with
+  | H: anno _ _ _ _ _ = _,
+    H1: anno _ _ _ _ _ = _ |- _ => 
+    eapply anno_aeval in H as ?;
+    eapply anno_aeval in H1 as ?;
+    repeat find_rewrite;
+    repeat find_injection;
+    ffa
   end.
+Qed.
 
 Lemma eval_aeval:
-  forall t t' p e i i' G cm,
-    anno G e t i = resultC (i', t') ->
-    eval G cm t p e = aeval G cm t' p e.
+  forall t t' p e i i' G e',
+    anno G p e t i = resultC (i', t', e') ->
+    eval G p e t = aeval G p e t'.
 Proof.
-  induction t; simpl in *; 
-  intuition; eauto; ff;
-  result_monad_unfold; ff;
-  result_monad_unfold; ff; 
-  rw; eauto.
-  result_monad_unfold; ff.
-  - eapply IHt; rw; eauto.
-  - erewrite IHt1; eauto; rw;
-    result_monad_unfold; ff;
-    eapply IHt2; rw; eauto.
-  - erewrite IHt1; eauto; rw;
-    erewrite IHt2; eauto; rw;
-    eauto.
-  - erewrite IHt1; eauto; rw;
-    erewrite IHt2; eauto; rw;
-    eauto.
+  intros;
+  eapply anno_eval in H as ?;
+  eapply anno_aeval in H as ?;
+  ff.
 Qed.
 
 (** This predicate determines if an annotated term is well formed,
     that is if its ranges correctly capture the relations between a
     term and its associated events. *)
-Inductive well_formed_r_annt
-    : ASP_Type_Env -> EvidenceT -> AnnoTerm -> Prop :=
-| wf_asp_r_annt: forall r e x G n,
+Inductive well_formed_r_annt : GlobalContext -> AnnoCopPhrase -> Prop :=
+| wf_asp_r_annt: forall r e x G n p,
     match x with 
     | APPR => et_size G e 
     | _ => resultC 0 end = resultC n ->
     snd r = S (fst r) + n ->
-    well_formed_r_annt G e (aasp r x)
+    well_formed_r_annt G (anno_cop_phrase p e (aasp r x))
 
-| wf_att_r_annt: forall r p x e G,
-    well_formed_r_annt G e x ->
+| wf_att_r_annt: forall r p x e G p',
+    well_formed_r_annt G (anno_cop_phrase p' e x) ->
     S (fst r) = fst (range x) ->
     snd r = S (snd (range x)) ->
     Nat.pred (snd r) > fst r ->
-    well_formed_r_annt G e (aatt r p x)               
+    well_formed_r_annt G (anno_cop_phrase p e (aatt r p' x))
 
-| wf_lseq_r_annt: forall r x y e G,
-    well_formed_r_annt G e x -> 
-    well_formed_r_annt G e y ->
+| wf_lseq_r_annt: forall r x y e G p e',
+    well_formed_r_annt G (anno_cop_phrase p e x) ->
+    aeval G p e x = resultC e' ->
+    well_formed_r_annt G (anno_cop_phrase p e' y) ->
     fst r = fst (range x) ->
     snd (range x) = fst (range y) ->
     snd r = snd (range y) -> 
-    well_formed_r_annt G e (alseq r x y)               
+    well_formed_r_annt G (anno_cop_phrase p e (alseq r x y))
 
-| wf_bseq_r_annt: forall r s x y e G,
-    well_formed_r_annt G e x -> 
-    well_formed_r_annt G e y ->
+| wf_bseq_r_annt: forall r s x y e G p,
+    well_formed_r_annt G (anno_cop_phrase p (splitEv_T_l s e) x) -> 
+    well_formed_r_annt G (anno_cop_phrase p (splitEv_T_r s e) y) ->
     S (fst r) = fst (range x) ->
     snd (range x) = fst (range y) ->
     snd r = S (snd (range y)) ->  
-    well_formed_r_annt G e (abseq r s x y)              
+    well_formed_r_annt G (anno_cop_phrase p e (abseq r s x y))
 
-| wf_bpar_r_annt: forall r s x y e G,
-    well_formed_r_annt G e x -> 
-    well_formed_r_annt G e y ->  
+| wf_bpar_r_annt: forall r s x y e G p,
+    well_formed_r_annt G (anno_cop_phrase p (splitEv_T_l s e) x) -> 
+    well_formed_r_annt G (anno_cop_phrase p (splitEv_T_r s e) y) ->
     S (fst r) = fst (range x) ->
     snd (range x) = fst (range y) ->
     (snd r) = S (snd (range y)) ->
     (*fst (range y) > fst (range x) -> *)
-    well_formed_r_annt G e (abpar r s x y).
+    well_formed_r_annt G (anno_cop_phrase p e (abpar r s x y)).
 #[export] Hint Constructors well_formed_r_annt : core.
 
-
-Lemma same_anno_range: forall t i a b e n n',
-    anno e t i = (n,a) ->
-    anno e t i = (n',b) ->
-    n = n'.
-Proof.
-  intros; find_rewrite; find_injection; eauto.
-Qed.
-
-Lemma anno_ev_mono : forall e i,
-  anno_ev e i > i.
-Proof.
-  induction e; simpl in *; intros; try lia.
-  - pose proof (IHe i); lia. 
-  - pose proof (IHe1 i);
-    pose proof (IHe2 (anno_ev e1 i)); lia.
-Qed.
-
-Lemma anno_mono : forall (t:Term) (i j:nat) (t':AnnoTerm) e,
-  anno e t i = (j,t') ->
+Lemma anno_mono : forall (t:Term) (i j:nat) (t':AnnoTerm) e e' G p,
+  anno G p e t i = resultC (j,t',e') ->
   j > i.
 Proof.
-  induction t; intuition; ffa; try lia;
-  eapply anno_ev_mono.
+  induction t; intuition; ffa using (result_monad_unfold; try lia).
 Qed.
 #[export] Hint Resolve anno_mono : core.
 
 Lemma anno_range:
-  forall x i j t' e,
-    anno e x i = (j,t') ->
+  forall x i j t' e G e' p,
+    anno G p e x i = resultC (j, t',e') ->
     range (t') = (i, j).
 Proof.
-  induction x; intros; ff.
+  induction x; intros; ffa using result_monad_unfold.
 Qed.
-
 
 (** Lemma stating that any annotated term produced via anno is well formed *)
 Lemma anno_well_formed_r:
-  forall t i j t' G e,
-    anno e t i = (j, t') ->
-    well_formed_r_annt G e t'.
+  forall t i j t' G e e' p,
+    anno G p e t i = resultC (j, t', e') ->
+    well_formed_r_annt G (anno_cop_phrase p e t').
 Proof.
-  induction t; intros; ff;
-  try (econstructor; ff;
-  try (repeat find_apply_lem_hyp anno_range;
-    repeat find_rewrite; ff; fail); 
-    try assert (n > S i) by eauto; lia).
-  econstructor; simpl in *.
+  induction t; intros; eauto.
+  - ffa using result_monad_unfold.
+  - simpl in *; result_monad_unfold;
+    ff.
+    econstructor; simpl in *; eauto;
+    try (find_apply_lem_hyp anno_range;
+    find_rewrite; simpl in *; eauto).
+    assert (n > S i) by eauto;
+    simpl in *; lia.
+  - simpl in *; result_monad_unfold;
+    ff; econstructor; eauto;
+    try (repeat find_apply_lem_hyp anno_range;
+      repeat find_rewrite;
+      simpl in *; eauto; fail).
+    eapply IHt1 in Heqr as ?;
+    eapply anno_aeval in Heqr as ?;
+    repeat find_rewrite; ff.
+  - simpl in *; result_monad_unfold;
+    ff; econstructor; eauto;
+    try (repeat find_apply_lem_hyp anno_range;
+      repeat find_rewrite;
+      simpl in *; eauto; fail).
+  - simpl in *; result_monad_unfold;
+    ff; econstructor; eauto;
+    try (repeat find_apply_lem_hyp anno_range;
+      repeat find_rewrite;
+      simpl in *; eauto; fail).
 Qed.
 
 (* Computes the length of the "span" or range of event IDs for a given Term *)
-Fixpoint event_id_span_Term (t: Term) : nat :=
+Fixpoint event_id_span_Term (G : GlobalContext) (p : Plc) (e : EvidenceT) (t: Term) 
+    : ResultT nat string :=
   match t with
-  | asp x => 1
-  | att p x => 2 + (event_id_span_Term x)
-  | lseq x y => (event_id_span_Term x) + (event_id_span_Term y)
-  | bseq s x y => 2 + (event_id_span_Term x) + (event_id_span_Term y)
-  | bpar s x y => 2 + (event_id_span_Term x) + (event_id_span_Term y)
+  | asp x => 
+    match x with
+    | APPR => match et_size G e with
+              | errC s => errC s
+              | resultC n => resultC (1 + n)
+              end
+    | _ => resultC 1
+    end
+  | att p x => 
+    n' <- (event_id_span_Term G p e x) ;;
+    resultC (2 + n')
+  | lseq x y => 
+    n1 <- (event_id_span_Term G p e x) ;;
+    e' <- eval G p e x ;;
+    n2 <- (event_id_span_Term G p e' y) ;;
+    resultC (n1 + n2)
+  | bseq s x y => 
+    n1 <- (event_id_span_Term G p (splitEv_T_l s e) x) ;;
+    n2 <- (event_id_span_Term G p (splitEv_T_r s e) y) ;;
+    resultC (2 + n1 + n2)
+  | bpar s x y => 
+    n1 <- (event_id_span_Term G p (splitEv_T_l s e) x) ;;
+    n2 <- (event_id_span_Term G p (splitEv_T_r s e) y) ;;
+    resultC (2 + n1 + n2)
   end.
 
-(* Same as event_id_span', but for Core Terms *)
-Fixpoint event_id_span_Core (t: Core_Term) : nat :=
-  match t with
-  | aspc CLEAR => 0
-  | attc _ x => 2 + (event_id_span_Term x)
-  | lseqc x y => (event_id_span_Core x) + (event_id_span_Core y)
-  | bseqc x y => 2 + (event_id_span_Core x) + (event_id_span_Core y)
-  | bparc _ x y => 2 + (event_id_span_Core x) + (event_id_span_Core y)
-  | _ => 1
-  end.
-
-Lemma event_id_works : forall t,
-  event_id_span_Term t = event_id_span_Core (copland_compile t).
-Proof with (simpl in *; eauto).
-  induction t...
-  - destruct a... destruct s...
-  - destruct s, s, s0...
-  - destruct s, s, s0...
-Qed.
-
-
-Lemma span_range : forall t i j t',
-  anno t i = (j, t') ->
-  event_id_span_Term t = (j - i).
+Lemma span_range : forall G t t' p i i' e e',
+  anno G p e t i = resultC (i', t', e') ->
+  event_id_span_Term G p e t = resultC (i' - i).
 Proof.
   intros.
   generalizeEverythingElse t.
-  induction t; intros; simpl in *; try find_injection; try lia;
-  ff; repeat match goal with
-  | H: anno _ _ = _ ,
-    IH : context[forall _, anno _ _ = _ -> _] |- _  => 
-    let H' := fresh "H" in
-    pose proof H as H'; apply anno_mono in H';
-    eapply IH in H; eauto;
-    repeat find_rewrite
-  end; lia. 
+  induction t; intros; simpl in *; try find_injection; try lia.
+  - break_match; simpl in *; try find_injection; try (f_equal; lia);
+    result_monad_unfold;
+    break_match; try congruence; 
+    repeat find_injection; try (f_equal; lia);
+    break_match; try congruence;
+    repeat find_injection; f_equal; lia.
+  - result_monad_unfold; ff;
+    match goal with
+    | H : anno _ _ _ _ _ = _ |- _ => 
+      eapply anno_mono in H as ?
+    end; ffa;
+    repeat find_rewrite; repeat find_injection;
+    try (f_equal; lia).
+  - result_monad_unfold; ff;
+    match goal with
+    | H : anno _ _ _ t1 _ = _,
+      H1 : anno _ _ _ t2 _ = _ |- _ => 
+      eapply anno_mono in H as ?;
+      eapply anno_mono in H1 as ?;
+      eapply anno_aeval in H as ?;
+      eapply anno_aeval in H1 as ?;
+      eapply eval_aeval in H as ?;
+      eapply eval_aeval in H1 as ?;
+      eapply IHt1 in H;
+      eapply IHt2 in H1
+    end; ffa; repeat find_rewrite; 
+    repeat find_injection;
+    repeat find_rewrite; repeat find_injection;
+    try (f_equal; lia).
+  - result_monad_unfold; ff;
+    match goal with
+    | H : anno _ _ _ t1 _ = _,
+      H1 : anno _ _ _ t2 _ = _ |- _ => 
+      eapply anno_mono in H as ?;
+      eapply anno_mono in H1 as ?;
+      eapply anno_aeval in H as ?;
+      eapply anno_aeval in H1 as ?;
+      repeat find_rewrite; repeat find_injection;
+      eapply eval_aeval in H as ?;
+      eapply eval_aeval in H1 as ?;
+      eapply IHt1 in H;
+      repeat find_rewrite; 
+      repeat find_injection; try congruence;
+      eapply IHt2 in H1;
+      repeat find_rewrite; 
+      repeat find_injection; try congruence
+    end;
+    repeat find_injection;
+    repeat find_rewrite; repeat find_injection;
+    try congruence;
+    try (f_equal; lia).
+  - result_monad_unfold; ff;
+    match goal with
+    | H : anno _ _ _ t1 _ = _,
+      H1 : anno _ _ _ t2 _ = _ |- _ => 
+      eapply anno_mono in H as ?;
+      eapply anno_mono in H1 as ?;
+      eapply anno_aeval in H as ?;
+      eapply anno_aeval in H1 as ?;
+      repeat find_rewrite; repeat find_injection;
+      eapply eval_aeval in H as ?;
+      eapply eval_aeval in H1 as ?;
+      eapply IHt1 in H;
+      repeat find_rewrite; 
+      repeat find_injection; try congruence;
+      eapply IHt2 in H1;
+      repeat find_rewrite; 
+      repeat find_injection; try congruence
+    end;
+    repeat find_injection;
+    repeat find_rewrite; repeat find_injection;
+    try congruence;
+    try (f_equal; lia).
 Qed.
